incredibly hard.

src/SSmty.v
@@ -97,8 +97,8 @@ Inductive tm : Set :=
 
 Inductive subty  : ty -> ty -> Prop :=
 | stfun : forall x x' y y',
-            subty x x' ->
-            subty y' y ->
+            subty x' x ->
+            subty y y' ->
             subty (TFun x y) (TFun x' y')
 | stsum : forall x x' y y',
             subty x x' ->
@@ -126,6 +126,30 @@ Inductive subty  : ty -> ty -> Prop :=
             subty t0 t2.
 
     Hint Constructors subty.
+
+    Ltac destructALL :=
+    repeat (
+        match goal with
+        | h0: _ \/ _ |- _ => destruct h0
+        | h0: _ /\ _ |- _ => destruct h0
+        | h0: exists _, _ |- _ => destruct h0
+        | h0: {_ | _} |- _ => destruct h0
+        | h0: {_} + {_} |- _ => destruct h0
+        | h0: _ + {_} |- _ => destruct h0
+        | h0: _ + _ |- _ => destruct h0
+        end
+    ).
+
+Theorem subty_wf:
+    forall a b,
+        subty a b ->
+        wf_ty a /\ wf_ty b.
+    
+    intros.
+    induction H; intros; subst;
+    try (destructALL; subst; eauto;fail).
+Qed.
+
     
 Theorem only_rcd_dec:
     forall T,
@@ -286,74 +310,28 @@ Theorem eq_ty_dec:
     try (right; intro hhhh; inversion hhhh; subst; eauto; fail).
 Qed.
 
-Definition subty_dec_alg:
-    forall (T1 T2: ty),
-        bool.
-    intros T1 T2.
-    remember T1 as T1'; remember T2 as T2'.
-    symmetry in HeqT1'. symmetry in HeqT2'.
-    generalize dependent T2. generalize dependent T1.
-    generalize dependent T2'.
-    induction T1';
-    intros T2';
-    induction T2';
-    try(
-    intros T1 h0 T2 h1;
-    match goal with
-    | h0 : T1 = TNat, h1 :T2 = TNat |- _ =>
-        apply true
-    | h0 : T1 = TBool, h1 :T2 = TBool |- _ =>
-        apply true
-    | h0 : T1 = TChr, h1 : T2 = TChr |- _ =>
-        apply true
-    | h0 : T1 = TNone, h1: T2 = TNone |- _ =>
-        apply true
-    | h0: T1 = (TRcons _ _ _), h1: T2 = TNone |- _ =>
-        apply true
-    | |- _ => idtac
-    end; 
-    match goal with
-    | h0 : _ = TNat |- _ =>
-        apply false
-    | h0 : _ = TBool |- _ =>
-        apply false
-    | h0 : _ = TChr |- _ =>
-        apply false
-    | h1: T1 = TNone |- _ =>
-        apply false
-    | |- _ => idtac
-    end;
-    match goal with
-    | h0 : T1 = (?TF ?T0 ?T1),
-      h1 : T2 = (?TF ?T0' ?T1'),
-      h2 : forall (_ _: ty), _ = ?T0 ->
-            forall _, _ = _ -> bool,
-      h3 : forall (_ _: ty), _ = ?T1 ->
-            forall _, _ = _ -> bool |- _ =>
-        destruct (h2 T0' _ eq_refl _ eq_refl) eqn: hhh0;
-        destruct (h2 T1' _ eq_refl _ eq_refl) eqn: hhh1;
-        match goal with
-        | ha : _ = true, hb : _ = true |- _ =>
-            apply true
-        | |- _ => apply false
-        end
-    | h0 : T1 = (TRcons _ ?T0 ?T1),
-      h1 : T2 = (TRcons _ ?T0' ?T1') |- _ =>
-        idtac
-    | |- _ => apply false
-    end;
-    fail
-    ).
-    (* The only case left, TRCons, width & depth*)
-    intros.
-    destruct (IHT1'1 T2 _ eq_refl _ eq_refl) eqn:h1.
+Definition eq_ty_bool (T1 T2: ty) : bool.
+    destruct (eq_ty_dec T1 T2).
     apply true.
-    destruct (IHT1'1 T2'1 _ eq_refl _ eq_refl) eqn:h2.
-    destruct (IHT1'2 T2'2 _ eq_refl _ eq_refl) eqn:h3.
-    apply true.
-    apply false.
     apply false.
 Defined.
+
+
+(*Fixpoint subty_dec_alg (T1 T2 : ty) {struct T1}: bool :=
+    orb (eq_ty_bool T1 T2)
+        (
+            match T1, T2 with
+            | (TFun x0 y0), (TFun x1 y1) =>
+            andb (subty_dec_alg x1 x0) (subty_dec_alg y0 y1)
+            | (TSum x0 y0), (TSum x1 y1) => 
+            andb (subty_dec_alg x0 x1) (subty_dec_alg y0 y1)
+            | TRcons _ _ _, TNone => true
+            | (TRcons _ x0 y0), (TRcons i x1 y1) => 
+            orb (andb (subty_dec_alg x0 x1) (subty_dec_alg y0 y1))
+                (subty_dec_alg y0 (TRcons i x1 y1))
+            | _, _ => false
+            end
+).*)
 
 Lemma subty_onlyrefl_tnat1:
     forall T,
@@ -521,22 +499,108 @@ Qed.
 
 
 
+Lemma subty_extra_tfun:
+    forall x y x' y',
+        subty (TFun x y) (TFun x' y') ->
+        subty x' x /\ subty y y'.
+    
+    intros.
+    remember (TFun x y) as T.
+    remember (TFun x' y') as T'.
+    generalize dependent x.
+    generalize dependent y.
+    generalize dependent x'.
+    generalize dependent y'.
+    induction H; intros; subst;
+    try discriminate;
+    try (split; eauto; fail).
+    inversion HeqT';
+    inversion HeqT; subst. tauto.
+    inversion HeqT; inversion H; subst; eauto.
+    destruct (subty_extrac_tfun0 _ _ _ H).
+    destruct (subty_extrac_tfun1 _ _ _ H0).
+    destructALL. subst. inversion H2; subst; eauto.
+    destruct (IHsubty1 _ _ eq_refl _ _ eq_refl).
+    destruct (IHsubty2 _ _ eq_refl _ _ eq_refl).
+    split; eauto.
+Qed.
 
-(*Lemma subty_ext_fun:
-    forall T1 T1' T2 T2',
-        subty (TFun T1 T2) (TFun T1' T2') ->
-        subty T1 T1' /\ subty T2 T2'.*)
+Lemma subty_extra_tsum:
+    forall x y x' y',
+        subty (TSum x y) (TSum x' y') ->
+        subty x x' /\ subty y y'.
+    
+    intros.
+    remember (TSum x y) as T.
+    remember (TSum x' y') as T'.
+    generalize dependent x.
+    generalize dependent y.
+    generalize dependent x'.
+    generalize dependent y'.
+    induction H; intros; subst;
+    try discriminate;
+    try (split; eauto; fail).
+    inversion HeqT';
+    inversion HeqT; subst. tauto.
+    inversion HeqT; inversion H; subst; eauto.
+    destruct (subty_extrac_tsum0 _ _ _ H).
+    destruct (subty_extrac_tsum1 _ _ _ H0).
+    destructALL. subst. inversion H2; subst; eauto.
+    destruct (IHsubty1 _ _ eq_refl _ _ eq_refl).
+    destruct (IHsubty2 _ _ eq_refl _ _ eq_refl).
+    split; eauto.
+Qed.
 
-Theorem subty_dec:
+Ltac general_val_ X u v :=
+    match v with
+      | 0 => X;(generalize dependent u)
+      | _ => general_val_ ltac:(X; generalize dependent u) v
+    end.
+
+Ltac glize :=
+    general_val_ idtac.
+
+Lemma subty_rcons_none:
+    forall i head tail T,
+        T = TRcons i head tail ->
+        wf_ty T ->
+        only_rcd T ->
+        subty T TNone.
+    intros i head tail T h0 h1 h2.
+    glize i head tail h1 0.
+    induction h2; subst; eauto.
+    intros. inversion h0; subst; eauto; inversion h1; subst; eauto.
+    eapply strcdw;eauto.
+    destruct h2; eauto.
+Qed.
+
+  
+
+Axiom wf_ty_rcons_rcd:
+    forall i T1 T2,
+        wf_ty (TRcons i T1 T2) ->
+        only_rcd T2.
+(* I don't know how the fuck this is happening
+    I will try to make only_rcd into prop again.
+*)
+
+Theorem subty_dec_compl:
     forall T1 T2,
-        {subty T1 T2} + {~ subty T1 T2}.
+        {subty T1 T2 /\ subty T2 T1} +
+        {subty T1 T2 /\ ~subty T2 T1} +
+        {~subty T1 T2 /\ subty T2 T1} +
+        {~subty T1 T2 /\ ~subty T2 T1}.
+
+    Ltac fst := left; left; left.
+    Ltac snd := left; left; right.
+    Ltac trd := left; right.
+    Ltac fth := right.
 
     intros T1;
     induction T1;
-    intros T2;
-    induction T2;
+    intros T2; induction T2;
     try (
-        right; intro;
+        fth; split; intro;
         match goal with
         | h0 : subty TNat _ |- _ =>
             poses' (subty_onlyrefl_tnat0 _ h0); eauto
@@ -553,21 +617,95 @@ Theorem subty_dec:
         | h0 : subty TNone _ |- _ =>
             poses' (subty_onlyrefl_tnone0 _ h0); eauto
         | h0 : subty (TFun _ _) _ |- _ =>
-            poses' (subty_extrac_tfun0 _ h0); destructALL; eauto
-        | h0 : subty (TFun _ _) _ |- _ =>
-            poses' (subty_extrac_tfun0 _ h0); destructALL; eauto
+            poses' (subty_extrac_tfun0 _ _ _ h0); destructALL; eauto
+        | h0 : subty _ (TFun _ _) |- _ =>
+            poses' (subty_extrac_tfun1 _ _ _ h0); destructALL; eauto
+        | h0 : subty (TSum _ _) _ |- _ =>
+            poses' (subty_extrac_tsum0 _ _ _ h0); destructALL; eauto
+        | h0 : subty _ (TSum _ _) |- _ =>
+            poses' (subty_extrac_tsum1 _ _ _ h0); destructALL; eauto
         end; try discriminate; fail
     );
     try (
-        left; eauto; fail
-    );
-    try (
-        match goal with
-        | |- {_} + {}
-    )
+        fst; eauto; fail
+    ).
+    
+    
+    Ltac extra_tcombine :=
+        repeat (match goal with
+        | h0 : subty (TFun _ _) (TFun _ _) |- _ =>
+            poses' (subty_extra_tfun _ _ _ _ h0);
+            generalize dependent h0;
+            destructALL
+        | h0 : subty (TSum _ _) (TSum _ _) |- _ =>
+            poses' (subty_extra_tsum _ _ _ _ h0);
+            generalize dependent h0;
+            destructALL
+        end); intros.
+    (* case tfun *)
+    clear IHT2_1. clear IHT2_2.
+    poses' (IHT1_1 T2_1);
+    poses' (IHT1_2 T2_2);
+    destructALL;
+    try (fst; split; eauto; fail);
+    try (snd; split; eauto; 
+        try (intro h0; extra_tcombine; subst; eauto; fail);
+        fail);
+    try (trd; split; eauto;
+        try (intro h0; extra_tcombine; subst; eauto; fail);
+        fail);
+    try (fth; split; eauto;
+        try (intro h0; extra_tcombine; subst; eauto; fail);
+        fail).
 
+    (* case tsum *)
 
+    clear IHT2_1. clear IHT2_2.
+    poses' (IHT1_1 T2_1);
+    poses' (IHT1_2 T2_2);
+    destructALL;
+    try (fst; split; eauto; fail);
+    try (snd; split; eauto; 
+        try (intro h0; extra_tcombine; subst; eauto; fail);
+        fail);
+    try (trd; split; eauto;
+        try (intro h0; extra_tcombine; subst; eauto; fail);
+        fail);
+    try (fth; split; eauto;
+        try (intro h0; extra_tcombine; subst; eauto; fail);
+        fail).
 
+    (* case TRcons *)
+    destruct (wf_ty_dec (TRcons i T2_1 T2_2)).
+    trd; eauto. split. intro. poses' (subty_onlyrefl_tnone0 _ H). try discriminate.
+    eapply  subty_rcons_none; eauto.
+    poses' (wf_ty_rcons_rcd _ _ _ w).
+    eauto.
+    fth; split; intro; eauto. poses' (subty_onlyrefl_tnone0 _ H). try discriminate.
+    destruct (subty_wf _ _ H); eauto.
+    destruct (wf_ty_dec (TRcons i T1_1 T1_2)).
+    snd; eauto. split. eapply subty_rcons_none; eauto.
+    poses' (wf_ty_rcons_rcd _ _ _ w). eauto.
+    intro. poses' (subty_onlyrefl_tnone0 _ H). try discriminate.
+    fth; split; intro; eauto. destruct (subty_wf _ _ H); eauto.
+    poses' (subty_onlyrefl_tnone0 _ H). try discriminate.
+
+    clear IHT2_1. clear IHT2_2.
+    poses' (IHT1_1 T2_1);
+    poses' (IHT1_2 T2_2);
+    poses' (IHT1_2 (TRcons ))
+    destructALL;
+    try (fst; split; eauto; fail);
+    try (snd; split; eauto; 
+        try (intro h0; extra_tcombine; subst; eauto; fail);
+        fail);
+    try (trd; split; eauto;
+        try (intro h0; extra_tcombine; subst; eauto; fail);
+        fail);
+    try (fth; split; eauto;
+        try (intro h0; extra_tcombine; subst; eauto; fail);
+        fail).
+    
 
 
 
